Examples/SmallListDemo.thy
@@ -22,15 +22,12 @@ apply (induction y)
 apply simp
 by simp
 
-fun rev :: "'a Lst \<Rightarrow> 'a Lst"
-where 
-  "rev Emp = Emp"
-| "rev (Cons x xs) = app (rev xs) (Cons x Emp)"
 
 fun len ::  "'a Lst \<Rightarrow> nat"
 where
   "len Emp = 0"
 | "len (Cons x xs) = 1 + (len xs)"  
+
 hipster app len
 lemma lemma_ab [thy_expl]: "len y + len z = len (app y z)"
 apply (induction y)
@@ -44,34 +41,15 @@ apply (metis lemma_a)
 apply simp
 by (metis SmallListDemo.lemma_ab Suc_eq_plus1_left add.left_commute len.simps(2))
 
-fun filt :: "('a \<Rightarrow> bool) \<Rightarrow> 'a Lst \<Rightarrow> 'a Lst" 
+
+
+fun rev :: "'a Lst \<Rightarrow> 'a Lst"
 where 
-  "filt p Emp = Emp"
-| "filt p (Cons x xs) = (if (p x) then (Cons x (filt p xs)) else (filt p xs))"
+  "rev Emp = Emp"
+| "rev (Cons x xs) = app (rev xs) (Cons x Emp)"
 
-fun mem :: "'a \<Rightarrow> 'a Lst \<Rightarrow> bool"
-where
-  "mem x Emp = False"
-| "mem x (Cons y ys) = ((x=y) \<or> (mem x ys))"
-
-hipster app filt
-lemma lemma_ad [thy_expl]: "filt y (filt y z) = filt y z"
-apply (induction z)
-apply simp
-by simp
-
-lemma lemma_ae [thy_expl]: "filt z (filt y x2) = filt y (filt z x2)"
-apply (induction x2)
-apply simp
-by simp
-
-lemma lemma_af [thy_expl]: "app (filt y z) (filt y x2) = filt y (app z x2)"
-apply (induction z)
-apply simp
-by simp
-
-hipster rev
-lemma lemma_ag [thy_expl]: "app (SmallListDemo.rev z) (SmallListDemo.rev y) =
+hipster rev len
+lemma lemma_ad [thy_expl]: "app (SmallListDemo.rev z) (SmallListDemo.rev y) =
 SmallListDemo.rev (app y z)"
 apply (induction y)
 apply simp
@@ -79,10 +57,94 @@ apply (metis lemma_a)
 apply simp
 by (metis lemma_aa)
 
-lemma lemma_ah [thy_expl]: "SmallListDemo.rev (SmallListDemo.rev y) = y"
+lemma lemma_ae [thy_expl]: "len (SmallListDemo.rev y) = len y"
 apply (induction y)
 apply simp
 apply simp
-by (metis Lst.distinct(1) SmallListDemo.rev.simps(1) SmallListDemo.rev.simps(2) app.elims app.simps(2) lemma_a lemma_ag)
+by (metis One_nat_def Suc_eq_plus1 Suc_eq_plus1_left lemma_ab len.simps(1) len.simps(2))
+
+lemma lemma_af [thy_expl]: "SmallListDemo.rev (SmallListDemo.rev y) = y"
+apply (induction y)
+apply simp
+apply simp
+by (metis Lst.distinct(1) SmallListDemo.rev.simps(1) SmallListDemo.rev.simps(2) app.elims app.simps(2) lemma_a lemma_ad)
+
+
+fun filt :: "('a \<Rightarrow> bool) \<Rightarrow> 'a Lst \<Rightarrow> 'a Lst" 
+where 
+  "filt p Emp = Emp"
+| "filt p (Cons x xs) = (if (p x) then (Cons x (filt p xs)) else (filt p xs))"
+
+hipster app filt
+lemma lemma_ag [thy_expl]: "filt y (filt y z) = filt y z"
+apply (induction z)
+apply simp
+by simp
+
+lemma lemma_ah [thy_expl]: "filt z (filt y x2) = filt y (filt z x2)"
+apply (induction x2)
+apply simp
+by simp
+
+lemma lemma_ai [thy_expl]: "app (filt y z) (filt y x2) = filt y (app z x2)"
+apply (induction z)
+apply simp
+by simp
+
+
+
+
+
+
+fun mem :: "'a \<Rightarrow> 'a Lst \<Rightarrow> bool"
+where
+  "mem x Emp = False"
+| "mem x (Cons y ys) = ((x=y) \<or> (mem x ys))"
+
+
+hipster mem rev
+lemma lemma_aj [thy_expl]: "mem y (app x2 (Lst.Cons z x3)) = mem y (Lst.Cons z (app x2 x3))"
+apply (induction x2)
+apply simp
+apply simp
+by (metis )
+
+lemma lemma_ak [thy_expl]: "mem y (app z (app z x2)) = mem y (app z x2)"
+apply (induction z)
+apply simp
+apply simp
+by (metis SmallListDemo.lemma_aj mem.simps(2))
+
+lemma lemma_al [thy_expl]: "mem y (app z (app x3 x2)) = mem y (app z (app x2 x3))"
+apply (induction x2)
+apply simp
+apply (metis lemma_a)
+apply simp
+by (metis Lst.distinct(1) Lst.inject SmallListDemo.lemma_aj app.elims lemma_aa mem.simps(2))
+
+lemma lemma_am [thy_expl]: "mem y (SmallListDemo.rev z) = mem y z"
+apply (induction z)
+apply simp
+apply simp
+by (metis lemma_a lemma_aj mem.simps(2))
+
+lemma lemma_an [thy_expl]: "mem y (app x2 z) = mem y (app z x2)"
+apply (induction x2)
+apply simp
+apply (metis lemma_a)
+apply simp
+by (metis SmallListDemo.lemma_aj mem.simps(2))
+
+lemma lemma_ao [thy_expl]: "mem y (app z (SmallListDemo.rev x2)) = mem y (app z x2)"
+apply (induction x2)
+apply simp
+apply simp
+by (metis SmallListDemo.rev.simps(1) SmallListDemo.rev.simps(2) lemma_a lemma_aa lemma_ad lemma_af lemma_al)
+
+
+
+
+
+
 
 end
