IsaHipster.thy
@@ -30,6 +30,7 @@ val haskell_path =
 (*val hipspec_cmd = haskell_path ^ "hipster-hipspec ";
 val hipspecifyer_cmd = haskell_path ^ "HipSpecifyer "; 
 *)
+
 val tipSpec_cmd = haskell_path ^ "tip-spec ";
 val tipTransl_cmd = haskell_path ^ "tip --hipster ";
 val tipGHC_cmd = haskell_path ^ "tip-ghc ";
